Proved pre-fancy barrett reduction correct (except 1 admit for bounds that are correct but for which bounds relaxation loses necessary information) and add explanatory comments.

src/Experiments/SimplyTypedArithmetic.v
@@ -8836,9 +8836,9 @@ Module PreFancy.
         match e with
         | Scalar _ s => Scalar s
         | LetInAppIdentZ _ t r idc x f =>
-          of_straightline_ident idc t r x (fun y => of_straightline (f y))
+          of_straightline_ident idc t r[0~>wordmax-1]%zrange x (fun y => of_straightline (f y))
         | LetInAppIdentZZ _ t r idc x f =>
-          of_straightline_ident idc t r x (fun y => of_straightline (f y))
+          of_straightline_ident idc t (r[0~>wordmax-1], r[0~>1])%zrange x (fun y => of_straightline (f y))
         end.
     End with_var.
 
@@ -8988,14 +8988,16 @@ Module PreFancy.
                      (word_range, flag_range)
                      (ident.Z.add_get_carry_concrete wordmax)
       | ok_addc :
-          forall c x y : scalar type.Z,
+          forall (c x y : scalar type.Z) outr,
             in_flag_range (get_range c) ->
             in_word_range (get_range x) ->
             in_word_range (get_range y) ->
+            lower outr = 0 ->
+            (0 <= upper (get_range c) + upper (get_range x) + upper (get_range y) <= upper outr \/ outr = word_range) ->
             ok_ident _
                      (type.prod type.Z type.Z)
                      (Pair (Pair c x) y)
-                     (word_range, flag_range)
+                     (outr, flag_range)
                      (ident.Z.add_with_get_carry_concrete wordmax)
       | ok_sub :
           forall x y : scalar type.Z,
@@ -9017,11 +9019,15 @@ Module PreFancy.
                      (word_range, flag_range)
                      (ident.Z.sub_with_get_borrow_concrete wordmax)
       | ok_rshi :
-          forall (x : scalar (type.prod type.Z type.Z)) n,
+          forall (x : scalar (type.prod type.Z type.Z)) n outr,
             in_word_range (fst (get_range x)) ->
             in_word_range (snd (get_range x)) ->
-            0 <= n < 2 * log2wordmax ->
-            ok_ident (type.prod type.Z type.Z) type.Z x word_range (ident.Z.rshi_concrete wordmax n)
+            (* note : using [outr] rather than [word_range] allows for cases where the result has been put in a smaller word size. *)
+            lower outr = 0 ->
+            0 <= n ->
+            ((0 <= (upper (snd (get_range x)) + upper (fst (get_range x)) * wordmax) / 2^n <= upper outr)
+              \/ outr = word_range) ->
+            ok_ident (type.prod type.Z type.Z) type.Z x outr (ident.Z.rshi_concrete wordmax n)
       | ok_selc :
           forall (x : scalar (type.prod type.Z type.Z)) (y z : scalar type.Z),
             in_flag_range (snd (get_range x)) ->
@@ -9078,14 +9084,16 @@ Module PreFancy.
       | ok_of_scalar : forall t s, ok_scalar s -> @ok_expr t (Scalar s)
       | ok_letin_z : forall s d r idc x f,
           ok_ident _ type.Z x r idc ->
+          (r <=? word_range)%zrange = true ->
           ok_scalar x ->
-          (forall y, has_range r y -> ok_expr (f y)) ->
+          (forall y, has_range (t:=type.Z) r y -> ok_expr (f y)) ->
           ok_expr (@LetInAppIdentZ _ _ s d r idc x f)
       | ok_letin_zz : forall s d r idc x f,
-          ok_ident _ (type.prod type.Z type.Z) x r idc ->
+          ok_ident _ (type.prod type.Z type.Z) x (r, flag_range) idc ->
+          (r <=? word_range)%zrange = true ->
           ok_scalar x ->
-          (forall y, has_range r y -> ok_expr (f y)) ->
-          ok_expr (@LetInAppIdentZZ _ _ s d r idc x f)
+          (forall y, has_range (t:=type.Z * type.Z) (r, flag_range) y -> ok_expr (f y)) ->
+          ok_expr (@LetInAppIdentZZ _ _ s d (r, flag_range) idc x f)
       .
 
       Ltac invert H :=
@@ -9205,14 +9213,25 @@ Module PreFancy.
         auto.
       Qed.
 
-      Lemma has_word_range_rshi n x y :
+      Lemma has_range_rshi r n x y :
         0 <= n ->
-        @has_range type.Z word_range (Z.rshi wordmax x y n).
+        0 <= x ->
+        0 <= y ->
+        lower r = 0 ->
+        (0 <= (y + x * wordmax) / 2^n <= upper r \/ r = word_range) ->
+        @has_range type.Z r (Z.rshi wordmax x y n).
       Proof.
         pose proof wordmax_gt_2.
-        intros; rewrite Z.rshi_correct by omega.
-        match goal with |- context [?x mod ?m] => pose proof (Z.mod_pos_bound x m ltac:(omega)) end.
-        cbn [has_range lower upper]; lia.
+        intros. cbv [has_range].
+        rewrite Z.rshi_correct by omega.
+        match goal with |- context [?x mod ?m] =>
+                        pose proof (Z.mod_pos_bound x m ltac:(omega)) end.
+        split; [lia|].
+        intuition.
+        { destruct (Z_lt_dec (upper r) wordmax); [ | lia].
+          rewrite Z.mod_small by (split; Z.zero_bounds; omega).
+          omega. }
+        { subst r. cbn [upper]. omega. }
       Qed.
 
       Lemma in_word_range_spec r :
@@ -9417,7 +9436,15 @@ Module PreFancy.
           autorewrite with to_div_mod.
           match goal with |- context[?x mod ?m] => pose proof (Z.mod_pos_bound x m ltac:(omega)) end.
           rewrite Z.div_between_0_if by omega.
-          split; break_match; lia. }
+          match goal with H : _ \/ _ |- _ => destruct H; subst end.
+          { split; break_match; try lia.
+            destruct (Z_lt_dec (upper outr) wordmax).
+            { match goal with |- _ <= ?y mod _ <= ?u =>
+                              assert (y <= u) by nia end.
+              rewrite Z.mod_small by omega. omega. }
+            { match goal with|- context [?x mod ?m] => pose proof (Z.mod_pos_bound x m ltac:(omega)) end.
+              omega. } }
+          { split; break_match; cbn; lia. } }
         {
           autorewrite with to_div_mod.
           match goal with |- context[?x mod ?m] => pose proof (Z.mod_pos_bound x m ltac:(omega)) end.
@@ -9429,7 +9456,12 @@ Module PreFancy.
           match goal with |- context[?x mod ?m] => pose proof (Z.mod_pos_bound x m ltac:(omega)) end.
           rewrite Z.div_sub_small by omega.
           split; break_match; lia. }
-        { apply has_word_range_rshi; omega. }
+        { apply has_range_rshi; try nia; [ ].
+          match goal with H : context [upper ?ra + upper ?rb * wordmax] |- context [?a + ?b * wordmax] =>
+                          assert ((a + b * wordmax) / 2^n <= (upper ra + upper rb * wordmax) / 2^n) by (apply Z.div_le_mono; Z.zero_bounds; nia)
+          end.
+          match goal with H : _ \/ ?P |- _ \/ ?P => destruct H; [left|tauto] end.
+          split; Z.zero_bounds; nia. }
         { rewrite Z.zselect_correct. break_match; omega. }
         { cbn [interp_scalar fst snd get_range] in *.
           rewrite Z.zselect_correct. break_match; omega. }
@@ -9529,20 +9561,34 @@ Module PreFancy.
             rewrite !Z.leb_refl; reflexivity. } }
       Qed.
 
-      Lemma of_straightline_ident_mul_correct t x y g :
+      Lemma halved_mul_range x y :
+        ok_scalar (Pair x y) ->
+        is_halved x ->
+        is_halved y ->
+        0 <= interp_scalar x * interp_scalar y < wordmax.
+      Proof.
+        intro Hok; invert Hok. intros.
+        repeat match goal with H : _ |- _ => apply is_halved_has_range in H; [|assumption] end.
+        cbv [has_range lower upper] in *.
+        pose proof half_bits_squared. nia.
+      Qed.
+
+      Lemma of_straightline_ident_mul_correct r t x y g :
         is_halved x ->
         is_halved y ->
         ok_scalar (Pair x y) ->
+        (word_range <=? r)%zrange = true ->
         @has_range type.Z word_range (ident.interp ident.Z.mul (interp_scalar (Pair x y))) ->
-        @interp interp_cast _ (of_straightline_ident dummy_arrow consts ident.Z.mul t word_range (Pair x y) g) =
+        @interp interp_cast _ (of_straightline_ident dummy_arrow consts ident.Z.mul t r (Pair x y) g) =
         @interp interp_cast _ (g (ident.interp ident.Z.mul (interp_scalar (Pair x y)))).
       Proof.
-        intros Hx Hy Hok ?; invert Hok; cbn [interp_scalar of_straightline_ident].
+        intros Hx Hy Hok ? ?; invert Hok; cbn [interp_scalar of_straightline_ident];
         destruct (is_halved_cases x Hx ltac:(assumption)) as [ [? [Pxlow [Pxhigh Pxi] ] ] | [? [Pxlow [Pxhigh Pxi] ] ] ];
           rewrite ?Pxlow, ?Pxhigh;
           destruct (is_halved_cases y Hy ltac:(assumption)) as [ [? [Pylow [Pyhigh Pyi] ] ] | [? [Pylow [Pyhigh Pyi] ] ] ];
           rewrite ?Pylow, ?Pyhigh;
-          cbn; rewrite Pxi, Pyi; rewrite interp_cast_noop by auto; reflexivity.
+          cbn; rewrite Pxi, Pyi; assert (0 <= interp_scalar x * interp_scalar y < wordmax) by (auto using halved_mul_range);
+            rewrite interp_cast_noop by (cbv [is_tighter_than_bool] in *; cbn [has_range upper lower] in *; rewrite andb_true_iff in *; intuition; Z.ltb_to_lt; lia); reflexivity.
       Qed.
 
       Lemma has_word_range_mod_small x:
@@ -9629,25 +9675,48 @@ Module PreFancy.
                  replace y with (fst y, snd y) by (destruct y; reflexivity)
         end; autorewrite with to_div_mod; solve [repeat (f_equal; try ring)].
 
-      Lemma of_straightline_ident_correct s d t x r (idc : ident.ident s d) g :
+      Fixpoint is_tighter_than_bool_range_type t : range_type t -> range_type t -> bool :=
+        match t with
+        | type.type_primitive type.Z => (fun r1 r2 => (r1 <=? r2)%zrange)
+        | type.prod a b => fun r1 r2 =>
+                             (is_tighter_than_bool_range_type a (fst r1) (fst r2))
+                               && (is_tighter_than_bool_range_type b (snd r1) (snd r2))
+        | _ => fun _ _ => true
+        end.
+
+      Definition range_ok {t} : range_type t -> Prop :=
+        match t with
+        | type.type_primitive type.Z => fun r => in_word_range r 
+        | type.prod type.Z type.Z => fun r => in_word_range (fst r) /\ snd r = flag_range
+        | _ => fun _ => False
+        end.
+
+      Lemma of_straightline_ident_correct s d t x r r' (idc : ident.ident s d) g :
         ok_ident s d x r idc ->
+        range_ok r' ->
+        is_tighter_than_bool_range_type d r r' = true ->
         ok_scalar x ->
-        @interp interp_cast _ (of_straightline_ident dummy_arrow consts idc t r x g) =
+        @interp interp_cast _ (of_straightline_ident dummy_arrow consts idc t r' x g) =
         @interp interp_cast _ (g (ident.interp idc (interp_scalar x))).
       Proof.
         intros.
         pose proof wordmax_half_bits_pos.
         pose proof (ident_interp_has_range _ _ x r idc ltac:(assumption) ltac:(assumption)).
-        induction H; try solve [auto using of_straightline_ident_mul_correct];
+        match goal with H : ok_ident _ _ _ _ _ |- _ => induction H end;
+          try solve [auto using of_straightline_ident_mul_correct];
+          cbv [is_tighter_than_bool_range_type is_tighter_than_bool range_ok] in *;
           cbn [of_straightline_ident ident.interp ident.gen_interp
                                      invert_selm invert_sell] in *;
             intros; rewrite ?Z.eqb_refl; cbn [andb];
             try match goal with |- context [invert_shift] => break_match end;
             cbn [interp interp_ident]; try destruct_scalar;
-            repeat match goal with
+          repeat match goal with
                    | _ => progress (cbn [fst snd interp_scalar] in * )
                    | _ => progress break_match; [ ]
                    | _ => progress autorewrite with zsimplify_fast
+                   | _ => progress Z.ltb_to_lt
+                   | H : _ /\ _ |- _ => destruct H
+                   | _ => rewrite andb_true_iff in *
                    | _ => rewrite interp_cast_noop with (r:=flag_range) in *
                        by (apply has_flag_range_cc_m'; auto; extract_ok_scalar)
                    | _ => rewrite interp_cast_noop with (r:=flag_range) in *
@@ -9662,10 +9731,10 @@ Module PreFancy.
                        by (eapply has_range_loosen;
                            [apply has_range_interp_scalar; extract_ok_scalar|];
                            assumption)
-                   | _ => rewrite interp_cast_noop by assumption
-                   | _ => rewrite interp_cast2_noop by assumption
+                   | _ => rewrite interp_cast_noop by (cbn [has_range fst snd] in *; split; lia)
+                   | _ => rewrite interp_cast2_noop by (cbn [has_range fst snd] in *; split; lia)
                    | _ => reflexivity
-                   end.
+                 end.
       Qed.
 
       Lemma of_straightline_correct {t} (e : expr t) :
@@ -9676,12 +9745,15 @@ Module PreFancy.
         induction 1; cbn [of_straightline]; intros;
           repeat match goal with
                  | _ => progress cbn [Straightline.expr.interp]
-                 | _ => rewrite of_straightline_ident_correct by auto
-                 | _ => rewrite interp_cast_noop by auto using ident_interp_has_range
-                 | _ => rewrite interp_cast2_noop by auto using ident_interp_has_range
-                 | H : forall y, has_range _ y -> interp _ = _ |- _ => rewrite H by auto using ident_interp_has_range
+                 | _ => erewrite of_straightline_ident_correct
+                     by (cbv [range_ok is_tighter_than_bool_range_type];
+                         eauto using in_word_range_word_range;
+                         try apply andb_true_iff; auto)
+                 | _ => rewrite interp_cast_noop by eauto using has_range_loosen, ident_interp_has_range
+                 | _ => rewrite interp_cast2_noop by eauto using has_range_loosen, ident_interp_has_range
+                 | H : forall y, has_range _ y -> interp _ = _ |- _ => rewrite H by eauto using has_range_loosen, ident_interp_has_range
                  | _ => reflexivity
-                 end.
+        end.
       Qed.
     End proofs.
 
@@ -9726,10 +9798,12 @@ Module PreFancy.
       Proof.
         induction 1; intros; cbn [of_straightline interp].
         { apply replace_interp_cast_scalar; auto. }
-        { rewrite !of_straightline_ident_correct by auto.
+        { erewrite !of_straightline_ident_correct by (eauto; cbv [range_ok]; apply in_word_range_word_range).
           rewrite replace_interp_cast_scalar with (interp_cast'0:=interp_cast') by auto.
           eauto using ident_interp_has_range. }
-        { rewrite !of_straightline_ident_correct by auto.
+        { erewrite !of_straightline_ident_correct by
+              (eauto; try solve [cbv [range_ok]; split; auto using in_word_range_word_range];
+               cbv [is_tighter_than_bool_range_type]; apply andb_true_iff; split; auto).
           rewrite replace_interp_cast_scalar with (interp_cast'0:=interp_cast') by auto.
           eauto using ident_interp_has_range. }
       Qed.
@@ -10248,6 +10322,34 @@ Module Prod.
                                             (Instr (SUB 0) lo (hi, y)
                                                    (Instr ADDM lo (lo, RegZero, RegMod)
                                                           (Ret lo))))))).
+
+  (* Barrett reduction -- this is only the "reduce" part, excluding the initial multiplication. *)
+  Definition MulMod x xHigh RegMuLow scratchp1 scratchp2 scratchp3 scratchp4 scratchp5 : @Fancy.expr register :=
+    let q1Bottom256 := scratchp1 in
+    let muSelect := scratchp2 in
+    let q2 := scratchp3 in
+    let q2High := scratchp4 in
+    let q2High2 := scratchp5 in
+    let q3 := scratchp1 in
+    let r2 := scratchp2 in
+    let r2High := scratchp3 in
+    let maybeM := scratchp1 in
+    Instr SELM muSelect (RegMuLow, RegZero)
+          (Instr (RSHI 255) q1Bottom256 (xHigh, x)
+                 (Mul256x256 q2 q2High q1Bottom256 RegMuLow scratchp5
+                             (Instr (RSHI 255) q2High2 (RegZero, xHigh)
+                                    (Instr (ADD 0) q2High (q2High, q1Bottom256)
+                                           (Instr (ADDC 0) q2High2 (q2High2, RegZero)
+                                                  (Instr (ADD 0) q2High (q2High, muSelect)
+                                                         (Instr (ADDC 0) q2High2 (q2High2, RegZero)
+                                                                (Instr (RSHI 1) q3 (q2High2, q2High)
+                                                                       (Mul256x256 r2 r2High RegMod q3 scratchp4
+                                                                                   (Instr (SUB 0) muSelect (x, r2)
+                                                                                          (Instr (SUBC 0) xHigh (xHigh, r2High)
+                                                                                                 (Instr SELL maybeM (RegMod, RegZero)
+                                                                                                        (Instr (SUB 0) q3 (muSelect, maybeM)
+                                                                                                               (Instr ADDM x (q3, RegZero, RegMod)
+                                                                                                                      (Ret x))))))))))))))).
 End Prod.
 
 Module ProdEquiv.
@@ -10434,6 +10536,74 @@ Module ProdEquiv.
       subst. cbn - [Z.add Z.modulo Z.testbit Z.mul Z.shiftl Fancy.lower128 Fancy.upper128].
       lia. }
   Qed.
+
+  Lemma mulll_comm rd x y cont cc ctx :
+    ProdEquiv.interp256 (Fancy.Instr Fancy.MUL128LL rd (x, y) cont) cc ctx = ProdEquiv.interp256 (Fancy.Instr Fancy.MUL128LL rd (y, x) cont) cc ctx.
+  Proof. rewrite !ProdEquiv.interp_step. cbn - [Fancy.interp]. rewrite Z.mul_comm. reflexivity. Qed.
+
+  Lemma mulhh_comm rd x y cont cc ctx :
+    ProdEquiv.interp256 (Fancy.Instr Fancy.MUL128UU rd (x, y) cont) cc ctx = ProdEquiv.interp256 (Fancy.Instr Fancy.MUL128UU rd (y, x) cont) cc ctx.
+  Proof. rewrite !ProdEquiv.interp_step. cbn - [Fancy.interp]. rewrite Z.mul_comm. reflexivity. Qed.
+
+  Lemma mullh_mulhl rd x y cont cc ctx :
+    ProdEquiv.interp256 (Fancy.Instr Fancy.MUL128LU rd (x, y) cont) cc ctx = ProdEquiv.interp256 (Fancy.Instr Fancy.MUL128UL rd (y, x) cont) cc ctx.
+  Proof. rewrite !ProdEquiv.interp_step. cbn - [Fancy.interp]. rewrite Z.mul_comm. reflexivity. Qed.
+
+  Lemma add_comm rd x y cont cc ctx :
+    0 <= ctx x < 2^256 ->
+    0 <= ctx y < 2^256 ->
+    ProdEquiv.interp256 (Fancy.Instr (Fancy.ADD 0) rd (x, y) cont) cc ctx = ProdEquiv.interp256 (Fancy.Instr (Fancy.ADD 0) rd (y, x) cont) cc ctx.
+  Proof.
+    intros; rewrite !ProdEquiv.interp_step. cbn - [Fancy.interp]. rewrite Z.add_comm.
+    rewrite !(Z.mod_small (ctx _)) by (cbn in *; omega). reflexivity.
+  Qed.
+
+  Lemma addc_comm rd x y cont cc ctx :
+    0 <= ctx x < 2^256 ->
+    0 <= ctx y < 2^256 ->
+    ProdEquiv.interp256 (Fancy.Instr (Fancy.ADDC 0) rd (x, y) cont) cc ctx = ProdEquiv.interp256 (Fancy.Instr (Fancy.ADDC 0) rd (y, x) cont) cc ctx.
+  Proof.
+    intros; rewrite !ProdEquiv.interp_step. cbn - [Fancy.interp]. rewrite (Z.add_comm (ctx x)).
+    rewrite !(Z.mod_small (ctx _)) by (cbn in *; omega). reflexivity.
+  Qed.
+
+  Ltac push_value_unused :=
+    repeat match goal with
+           | |- ~ In _ _ => cbn; intuition; congruence
+           | _ => apply ProdEquiv.value_unused_overwrite
+           | _ => apply ProdEquiv.value_unused_skip; [ | congruence | ]
+           | _ => apply ProdEquiv.value_unused_ret; congruence
+           end.
+
+  Ltac remember_single_result :=
+    match goal with |- context [(Fancy.spec ?i ?args ?cc) mod ?w] =>
+                    let x := fresh "x" in
+                    let y := fresh "y" in
+                    let Heqx := fresh "Heqx" in
+                    remember (Fancy.spec i args cc) as x eqn:Heqx;
+                    remember (x mod w) as y
+    end.
+  Ltac step_both_sides :=
+    match goal with |- ProdEquiv.interp256 (Fancy.Instr ?i ?rd1 ?args1 _) _ ?ctx1 = ProdEquiv.interp256 (Fancy.Instr ?i ?rd2 ?args2 _) _ ?ctx2 =>
+                    rewrite (ProdEquiv.interp_step i rd1 args1); rewrite (ProdEquiv.interp_step i rd2 args2);
+                    cbn - [Fancy.interp Fancy.spec];
+                    repeat progress rewrite ?reg_eqb_neq, ?reg_eqb_refl by congruence;
+                    remember_single_result;
+                    lazymatch goal with
+                    | |- context [Fancy.spec i _ _] =>
+                      let Heqa1 := fresh in
+                      let Heqa2 := fresh in
+                      remember (Tuple.map (n:=i.(Fancy.num_source_regs)) ctx1 args1) eqn:Heqa1;
+                      remember (Tuple.map (n:=i.(Fancy.num_source_regs)) ctx2 args2) eqn:Heqa2;
+                      cbn in Heqa1; cbn in Heqa2;
+                      repeat progress rewrite ?reg_eqb_neq, ?reg_eqb_refl in Heqa1 by congruence;
+                      repeat progress rewrite ?reg_eqb_neq, ?reg_eqb_refl in Heqa2 by congruence;
+                      let a1 := match type of Heqa1 with _ = ?a1 => a1 end in
+                      let a2 := match type of Heqa2 with _ = ?a2 => a2 end in
+                      (fail 1 "arguments to " i " do not match; LHS has " a1 " and RHS has " a2)
+                    | _ => idtac
+                    end
+    end.
 End ProdEquiv.
 
 (* Lemmas to help prove that a fancy and prefancy expression have the
@@ -11073,13 +11243,220 @@ Ltac solve_rbarrett_red_nocache := solve_rop_nocache BarrettReduction.rbarrett_r
 
 Module Barrett256.
 
-  Definition M := (2^256-2^224+2^192+2^96-1).
+  Definition M := Eval lazy in (2^256-2^224+2^192+2^96-1).
   Definition machine_wordsize := 256.
 
   Derive barrett_red256
          SuchThat (BarrettReduction.rbarrett_red_correctT M machine_wordsize barrett_red256)
          As barrett_red256_correct.
   Proof. Time solve_rbarrett_red machine_wordsize. Time Qed.
+
+  Definition muLow := Eval lazy in (2 ^ (2 * machine_wordsize) / M) mod (2^machine_wordsize).
+  Definition barrett_red256_prefancy' := PreFancy.of_Expr machine_wordsize [M; muLow] barrett_red256.
+
+  Derive barrett_red256_prefancy
+         SuchThat (barrett_red256_prefancy = barrett_red256_prefancy' type.interp)
+         As barrett_red256_prefancy_eq.
+  Proof. lazy - [type.interp]; reflexivity. Qed.
+
+  Lemma barrett_reduce_correct_specialized :
+    forall (xLow xHigh : Z),
+      0 <= xLow < 2 ^ machine_wordsize ->
+      0 <= xHigh < M ->
+      BarrettReduction.barrett_reduce machine_wordsize M muLow 2 2 xLow xHigh = (xLow + 2 ^ machine_wordsize * xHigh) mod M.
+  Proof.
+    intros.
+    apply BarrettReduction.barrett_reduce_correct; cbv [machine_wordsize M muLow] in *;
+      try omega;
+      try match goal with
+          | |- context [weight] => intros; cbv [weight]; autorewrite with zsimplify; auto using Z.pow_mul_r with omega
+          end; lazy; try split; congruence.
+  Qed.
+
+  (* Note: If this is not factored out, then for some reason Qed takes forever in barrett_red256_correct_full. *)
+  Lemma barrett_red256_correct_proj2 :
+    forall xy : type.interp (type.prod type.Z type.Z),
+      ZRange.type.option.is_bounded_by
+        (t:=type.prod type.Z type.Z)
+        (Some r[0 ~> 2 ^ machine_wordsize - 1]%zrange, Some r[0 ~> 2 ^ machine_wordsize - 1]%zrange)
+        xy = true ->
+       expr.Interp (@ident.interp) barrett_red256 xy = app_curried (t:=type.arrow (type.prod type.Z type.Z) type.Z) (fun xy => BarrettReduction.barrett_reduce machine_wordsize M muLow 2 2 (fst xy) (snd xy)) xy.
+  Proof. intros; destruct (barrett_red256_correct xy); assumption. Qed.
+  Lemma barrett_red256_correct_proj2' :
+    forall x y : Z,
+      ZRange.type.option.is_bounded_by
+        (t:=type.prod type.Z type.Z)
+        (Some r[0 ~> 2 ^ machine_wordsize - 1]%zrange, Some r[0 ~> 2 ^ machine_wordsize - 1]%zrange)
+        (x, y) = true ->
+       expr.Interp (@ident.interp) barrett_red256 (x, y) = BarrettReduction.barrett_reduce machine_wordsize M muLow 2 2 x y.
+  Proof. intros; rewrite barrett_red256_correct_proj2 by assumption; unfold app_curried; exact eq_refl. Qed.
+
+  Lemma barrett_red256_correct_full  :
+    forall (xLow xHigh : Z),
+      0 <= xLow < 2 ^ machine_wordsize ->
+      0 <= xHigh < M ->
+      expr.interp (@ident.interp) (barrett_red256 type.interp) (xLow, xHigh) = (xLow + 2 ^ machine_wordsize * xHigh) mod M.
+  Proof.
+    intros.
+    rewrite <-barrett_reduce_correct_specialized by assumption.
+    rewrite <-barrett_red256_correct_proj2'.
+    { cbv [expr.Interp type.uncurried_domain type.uncurry type.final_codomain].
+      reflexivity. }
+    { cbn. rewrite !andb_true_iff. cbv [machine_wordsize M] in *.
+      cbn in *. repeat split; apply Z.leb_le; omega. }
+  Qed.
+
+  (* TODO : maybe move these ok_expr tactics somewhere else *)
+  Ltac ok_expr_step' :=
+    match goal with
+    | _ => assumption
+    | |- _ <= _ <= _ \/ @eq zrange _ _ =>
+      right; lazy; try split; congruence
+    | |- _ <= _ <= _ \/ @eq zrange _ _ =>
+      left; lazy; try split; congruence
+    | |- context [PreFancy.ok_ident] => constructor
+    | |- context [PreFancy.ok_scalar] => constructor; try omega
+    | |- context [PreFancy.is_halved] => eapply PreFancy.is_halved_constant; [lazy; reflexivity | ]
+    | |- context [PreFancy.is_halved] => constructor
+    | |- context [PreFancy.in_word_range] => lazy; reflexivity
+    | |- context [PreFancy.in_flag_range] => lazy; reflexivity
+    | |- context [PreFancy.get_range] =>
+      cbn [PreFancy.get_range lower upper fst snd ZRange.map]
+    | x : type.interp (type.prod _ _) |- _ => destruct x
+    | |- (_ <=? _)%zrange = true =>
+      match goal with
+      | |- context [PreFancy.get_range_var] =>
+        cbv [is_tighter_than_bool PreFancy.has_range fst snd upper lower machine_wordsize M muLow] in *; cbn;
+        apply andb_true_iff; split; apply Z.leb_le
+      | _ => lazy
+      end; omega || reflexivity
+    | |- @eq zrange _ _ => lazy; reflexivity
+    | |- _ <= _ => cbv [machine_wordsize]; omega
+    | |- _ <= _ <= _ => cbv [machine_wordsize]; omega
+    end; intros.
+
+  (* TODO : maybe move these ok_expr tactics somewhere else *)
+  Ltac ok_expr_step :=
+    match goal with
+    | |- context [PreFancy.ok_expr] => constructor; cbn [fst snd]; repeat ok_expr_step'
+    end; intros; cbn [Nat.max].
+
+  Lemma barrett_red256_prefancy_correct :
+    forall xLow xHigh dummy_arrow,
+      0 <= xLow < 2 ^ machine_wordsize ->
+      0 <= xHigh < M ->
+      @PreFancy.interp machine_wordsize (PreFancy.interp_cast_mod machine_wordsize) type.Z (barrett_red256_prefancy (xLow, xHigh) dummy_arrow) = (xLow + 2 ^ machine_wordsize * xHigh) mod M.
+  Proof.
+    intros. rewrite barrett_red256_prefancy_eq; cbv [barrett_red256_prefancy'].
+    erewrite PreFancy.of_Expr_correct.
+    { apply barrett_red256_correct_full; try assumption; reflexivity. }
+    { reflexivity. }
+    { lazy; reflexivity. }
+    { lazy; reflexivity. }
+    { repeat constructor. }
+    { cbv [In M muLow]; intros; intuition; subst; cbv; congruence. }
+    { let r := (eval compute in (2 ^ machine_wordsize)) in
+      replace (2^machine_wordsize) with r in * by reflexivity.
+      cbv [M] in *.
+      assert (lower r[0~>1] = 0) by reflexivity.
+      repeat (ok_expr_step; [ ]).
+      ok_expr_step. { exact admit. (* TODO: the actual bounds on the second argument are lower, but relax_zrange steps have lost that information. *) }
+      repeat (ok_expr_step; [ ]).
+      ok_expr_step.
+      lazy; congruence.
+      constructor.
+      constructor. }
+    { lazy. omega. }
+  Qed.
+
+  Definition barrett_red256_fancy' (xLow xHigh RegMuLow RegMod RegZero error : positive) :=
+    Fancy.of_Expr 3%positive
+                  (fun z => if z =? muLow then Some RegMuLow else if z =? M then Some RegMod else if z =? 0 then Some RegZero else None)
+                  [M; muLow]
+                  barrett_red256
+                  (xLow, xHigh)%positive
+                  (fun _ _ => tt)
+                  error.
+  Derive barrett_red256_fancy
+         SuchThat (forall xLow xHigh RegMuLow RegMod RegZero,
+                      barrett_red256_fancy xLow xHigh RegMuLow RegMod RegZero = barrett_red256_fancy' xLow xHigh RegMuLow RegMod RegZero)
+         As barrett_red256_fancy_eq.
+  Proof.
+    intros.
+    lazy - [Fancy.ADD Fancy.ADDC Fancy.SUB Fancy.SUBC
+                      Fancy.MUL128LL Fancy.MUL128LU Fancy.MUL128UL Fancy.MUL128UU
+                      Fancy.RSHI Fancy.SELC Fancy.SELM Fancy.SELL Fancy.ADDM].
+    reflexivity.
+  Qed.
+
+  Import Fancy.Registers.
+
+  Definition barrett_red256_alloc' xLow xHigh RegMuLow :=
+    fun errorP errorR =>
+    Fancy.allocate register
+                   positive Pos.eqb
+                   errorR
+                   (barrett_red256_fancy 1000%positive 1001%positive 1002%positive 1003%positive 1004%positive errorP)
+                   [r2;r3;r4;r5;r6;r7;r8;r9;r10;r5;r11;r6;r12;r13;r14;r15;r16;r17;r18;r19;r20;r21;r22;r23;r24;r25;r26;r27;r28;r29]
+                   (fun n => if n =? 1000 then xLow
+                             else if n =? 1001 then xHigh
+                                  else if n =? 1002 then RegMuLow
+                                       else if n =? 1003 then RegMod
+                                            else if n =? 1004 then RegZero
+                                                 else errorR).
+  Derive barrett_red256_alloc
+         SuchThat (barrett_red256_alloc = barrett_red256_alloc')
+         As barrett_red256_alloc_eq.
+  Proof.
+    intros.
+    cbv [barrett_red256_alloc' barrett_red256_fancy].
+    cbn. subst barrett_red256_alloc.
+    reflexivity.
+  Qed.
+
+  Set Printing Depth 1000.
+  Import ProdEquiv.
+
+  Local Ltac solve_bounds :=
+    match goal with
+    | H : ?a = ?b mod ?c |- 0 <= ?a < ?c => rewrite H; apply Z.mod_pos_bound; omega
+    | _ => assumption
+    end.
+
+  Lemma barrett_red256_alloc_equivalent errorP errorR cc_start_state start_context :
+    forall x xHigh RegMuLow scratchp1 scratchp2 scratchp3 scratchp4 scratchp5 extra_reg,
+      NoDup [x; xHigh; RegMuLow; scratchp1; scratchp2; scratchp3; scratchp4; scratchp5; extra_reg; RegMod; RegZero] ->
+      0 <= start_context x < 2^machine_wordsize ->
+      0 <= start_context xHigh < 2^machine_wordsize ->
+      0 <= start_context RegMuLow < 2^machine_wordsize ->
+      ProdEquiv.interp256 (barrett_red256_alloc r0 r1 r30 errorP errorR) cc_start_state
+                          (fun r => if reg_eqb r r0
+                                    then start_context x
+                                    else if reg_eqb r r1
+                                         then start_context xHigh
+                                         else if reg_eqb r r30
+                                              then start_context RegMuLow
+                                              else start_context r)
+    = ProdEquiv.interp256 (Prod.MulMod x xHigh RegMuLow scratchp1 scratchp2 scratchp3 scratchp4 scratchp5) cc_start_state start_context.
+  Proof.
+    intros.
+    let r := eval compute in (2^machine_wordsize) in
+        replace (2^machine_wordsize) with r in * by reflexivity.
+    cbv [Prod.MulMod barrett_red256_alloc].
+
+    (* Extract proofs that no registers are equal to each other *)
+    repeat match goal with
+           | H : NoDup _ |- _ => inversion H; subst; clear H
+           | H : ~ In _ _ |- _ => cbv [In] in H
+           | H : ~ (_ \/ _) |- _ => apply Decidable.not_or in H; destruct H
+           | H : ~ False |- _ => clear H
+           end.
+
+    step_both_sides.
+
+    (* TODO: To prove equivalence between these two, we need to either relocate the RSHI instructions so they're in the same places or use instruction commutativity to push them down. *)
+
+  Admitted.
 
   Import PrintingNotations.
   Set Printing Width 1000.
@@ -11119,10 +11496,6 @@ barrett_red256 =  fun var : type -> Type => λ x : var (type.type_primitive type
                 ADDM (x27₁, 0, 115792089210356248762697446949407573530086143415290314195533631308867097853951)
      : Expr (type.uncurry (type.type_primitive type.Z -> type.type_primitive type.Z -> type.type_primitive type.Z))
   *)
-
-  Definition muLow := (2 ^ (2 * machine_wordsize) / M) mod (2^machine_wordsize).
-  Definition barrett_red256_prefancy :=
-    Eval lazy in (PreFancy.of_Expr machine_wordsize [M;muLow] barrett_red256).
 
   Import PreFancy.
   Import PreFancy.Notations.
@@ -11779,6 +12152,11 @@ Module Montgomery256.
   Ltac ok_expr_step' :=
     match goal with
     | _ => assumption
+    | |- _ <= _ <= _ \/ @eq zrange _ _ =>
+      right; lazy; try split; congruence
+    | |- _ <= _ <= _ \/ @eq zrange _ _ =>
+      left; lazy; try split; congruence
+    | |- lower r[0~>_]%zrange = 0 => reflexivity
     | |- context [PreFancy.ok_ident] => constructor
     | |- context [PreFancy.ok_scalar] => constructor; try omega
     | |- context [PreFancy.is_halved] => eapply PreFancy.is_halved_constant; [lazy; reflexivity | ]
@@ -11873,76 +12251,7 @@ Module Montgomery256.
     reflexivity.
   Qed.
 
-  (* TODO : move *)
-  Lemma mulll_comm rd x y cont cc ctx :
-    ProdEquiv.interp256 (Fancy.Instr Fancy.MUL128LL rd (x, y) cont) cc ctx = ProdEquiv.interp256 (Fancy.Instr Fancy.MUL128LL rd (y, x) cont) cc ctx.
-  Proof. rewrite !ProdEquiv.interp_step. cbn - [Fancy.interp]. rewrite Z.mul_comm. reflexivity. Qed.
-
-  Lemma mulhh_comm rd x y cont cc ctx :
-    ProdEquiv.interp256 (Fancy.Instr Fancy.MUL128UU rd (x, y) cont) cc ctx = ProdEquiv.interp256 (Fancy.Instr Fancy.MUL128UU rd (y, x) cont) cc ctx.
-  Proof. rewrite !ProdEquiv.interp_step. cbn - [Fancy.interp]. rewrite Z.mul_comm. reflexivity. Qed.
-
-  Lemma mullh_mulhl rd x y cont cc ctx :
-    ProdEquiv.interp256 (Fancy.Instr Fancy.MUL128LU rd (x, y) cont) cc ctx = ProdEquiv.interp256 (Fancy.Instr Fancy.MUL128UL rd (y, x) cont) cc ctx.
-  Proof. rewrite !ProdEquiv.interp_step. cbn - [Fancy.interp]. rewrite Z.mul_comm. reflexivity. Qed.
-
-  Lemma add_comm rd x y cont cc ctx :
-    0 <= ctx x < 2^256 ->
-    0 <= ctx y < 2^256 ->
-    ProdEquiv.interp256 (Fancy.Instr (Fancy.ADD 0) rd (x, y) cont) cc ctx = ProdEquiv.interp256 (Fancy.Instr (Fancy.ADD 0) rd (y, x) cont) cc ctx.
-  Proof.
-    intros; rewrite !ProdEquiv.interp_step. cbn - [Fancy.interp]. rewrite Z.add_comm.
-    rewrite !(Z.mod_small (ctx _)) by (cbn in *; omega). reflexivity.
-  Qed.
-
-  Lemma addc_comm rd x y cont cc ctx :
-    0 <= ctx x < 2^256 ->
-    0 <= ctx y < 2^256 ->
-    ProdEquiv.interp256 (Fancy.Instr (Fancy.ADDC 0) rd (x, y) cont) cc ctx = ProdEquiv.interp256 (Fancy.Instr (Fancy.ADDC 0) rd (y, x) cont) cc ctx.
-  Proof.
-    intros; rewrite !ProdEquiv.interp_step. cbn - [Fancy.interp]. rewrite (Z.add_comm (ctx x)).
-    rewrite !(Z.mod_small (ctx _)) by (cbn in *; omega). reflexivity.
-  Qed.
-
-  SearchAbout reg_eqb.
-
-  Local Ltac push_value_unused :=
-    repeat match goal with
-           | |- ~ In _ _ => cbn; intuition; congruence
-           | _ => apply ProdEquiv.value_unused_overwrite
-           | _ => apply ProdEquiv.value_unused_skip; [ | congruence | ]
-           | _ => apply ProdEquiv.value_unused_ret; congruence
-           end.
-
-  Local Ltac remember_single_result :=
-    match goal with |- context [(Fancy.spec ?i ?args ?cc) mod ?w] =>
-                    let x := fresh "x" in
-                    let y := fresh "y" in
-                    let Heqx := fresh "Heqx" in
-                    remember (Fancy.spec i args cc) as x eqn:Heqx;
-                    remember (x mod w) as y
-    end.
-  Local Ltac step_both_sides :=
-    match goal with |- ProdEquiv.interp256 (Fancy.Instr ?i ?rd1 ?args1 _) _ ?ctx1 = ProdEquiv.interp256 (Fancy.Instr ?i ?rd2 ?args2 _) _ ?ctx2 =>
-                    rewrite (ProdEquiv.interp_step i rd1 args1); rewrite (ProdEquiv.interp_step i rd2 args2);
-                    cbn - [Fancy.interp Fancy.spec];
-                    repeat progress rewrite ?reg_eqb_neq, ?reg_eqb_refl by congruence;
-                    remember_single_result;
-                    lazymatch goal with
-                    | |- context [Fancy.spec i _ _] =>
-                      let Heqa1 := fresh in
-                      let Heqa2 := fresh in
-                      remember (Tuple.map (n:=i.(Fancy.num_source_regs)) ctx1 args1) eqn:Heqa1;
-                      remember (Tuple.map (n:=i.(Fancy.num_source_regs)) ctx2 args2) eqn:Heqa2;
-                      cbn in Heqa1; cbn in Heqa2;
-                      repeat progress rewrite ?reg_eqb_neq, ?reg_eqb_refl in Heqa1 by congruence;
-                      repeat progress rewrite ?reg_eqb_neq, ?reg_eqb_refl in Heqa2 by congruence;
-                      let a1 := match type of Heqa1 with _ = ?a1 => a1 end in
-                      let a2 := match type of Heqa2 with _ = ?a2 => a2 end in
-                      (fail 1 "arguments to " i " do not match; LHS has " a1 " and RHS has " a2)
-                    | _ => idtac
-                    end
-    end.
+  Import ProdEquiv.
 
   Local Ltac solve_bounds :=
     match goal with
@@ -12170,143 +12479,19 @@ montred256 = fun var : type -> Type => (λ x : var (type.type_primitive type.Z *
 
 End Montgomery256.
 
-(* Extra-specialized ad-hoc pretty-printing *)
-Module FancyPrintingNotations.
-  Export ident.
-  Open Scope expr_scope.
-  Open Scope ctype_scope.
-  Notation "'RegMod'" :=
-    (AppIdent
-       (primitive 115792089210356248762697446949407573530086143415290314195533631308867097853951)
-       TT) (only printing, at level 9) : expr_scope.
-  Notation "'RegMuLow'" :=
-    (AppIdent
-       (primitive 26959946667150639793205513449348445388433292963828203772348655992835)
-       TT) (only printing, at level 9) : expr_scope.
-  Notation "'RegPinv'" :=
-    (AppIdent
-       (primitive 115792089210356248768974548684794254293921932838497980611635986753331132366849)
-       TT) (only printing, at level 9) : expr_scope.
-  Notation "'RegZero'" :=
-    (AppIdent
-       (primitive 0)
-       TT) (only printing, at level 9) : expr_scope.
-  Notation "'$R'" := 115792089237316195423570985008687907853269984665640564039457584007913129639936 : expr_scope.
-  Notation "'c.Lower(RegMod)'" :=
-    (AppIdent
-       (primitive 79228162514264337593543950335)
-       TT) (only printing, at level 9) : expr_scope.
-  Notation "'c.Upper(RegMod)'" :=
-    (AppIdent
-       (primitive 340282366841710300967557013911933812736)
-       TT) (only printing, at level 9) : expr_scope.
-  Notation "'c.Lower(RegMuLow)'" :=
-    (AppIdent
-       (primitive 340282366841710300930663525764514709507)
-       TT) (only printing, at level 9) : expr_scope.
-  Notation "'c.Upper(RegMuLow)'" :=
-    (AppIdent
-       (primitive 79228162514264337589248983038)
-       TT) (only printing, at level 9) : expr_scope.
-  Notation "'c.Lower(RegPinv)'" :=
-    (AppIdent
-       (primitive 79228162514264337593543950337)
-       TT) (only printing, at level 9) : expr_scope.
-  Notation "'c.Upper(RegPinv)'" :=
-    (AppIdent
-       (primitive 340282366841710300986003757985643364352)
-       TT) (only printing, at level 9) : expr_scope.
-  Notation "'uint256'"
-    := (r[0 ~> 115792089237316195423570985008687907853269984665640564039457584007913129639935]%zrange) : ctype_scope.
-  Notation "'uint128'"
-    := (r[0 ~> 340282366920938463463374607431768211455]%zrange) : ctype_scope.
-  Notation "$ n" := (Var n) (at level 10, format "$ n") : expr_scope.
-  Notation "$ n" := (Z.cast _ @@ Var n) (at level 10, format "$ n") : expr_scope.
-  Notation "$ n '_lo'" := (fst @@ (Var n))%expr (at level 10, format "$ n _lo") : expr_scope.
-  Notation "$ n '_hi'" := (snd @@ (Var n))%expr (at level 10, format "$ n _hi") : expr_scope.
-  Notation "$ n '_lo'" := (Z.cast _ @@ (fst @@ (Var n)))%expr (at level 10, format "$ n _lo") : expr_scope.
-  Notation "$ n '_hi'" := (Z.cast _ @@ (snd @@ (Var n)))%expr (at level 10, format "$ n _hi") : expr_scope.
-  Notation "$ n '_lo'" := (fst @@ (Z.cast2 _ @@ Var n))%expr (at level 10, format "$ n _lo") : expr_scope.
-  Notation "$ n '_hi'" := (snd @@ (Z.cast2 _ @@ Var n))%expr (at level 10, format "$ n _hi") : expr_scope.
-  Notation "$ n '_lo'" := (Z.cast _ @@ (fst @@ (Z.cast2 _ @@ Var n)))%expr (at level 10, format "$ n _lo") : expr_scope.
-  Notation "$ n '_hi'" := (Z.cast _ @@ (snd @@ (Z.cast2 _ @@ Var n)))%expr (at level 10, format "$ n _hi") : expr_scope.
-  Notation "'c.Mul128x128(' '$' n ',' x ',' y ');' f" :=
-    (expr_let n := Z.cast uint256 @@ (Z.mul @@ (x, y)) in
-         f)%expr (at level 40, f at level 200, right associativity, format "'[' 'c.Mul128x128(' '$' n ','  x ','  y ');' ']' '//' f") : expr_scope.
-  Notation "'c.Mul128x128(' '$' n ',' x ',' y ')' '<<' count ';' f" :=
-    (expr_let n := Z.cast _ @@ (Z.shiftl count @@ (Z.cast uint256 @@ (Z.mul @@ (x, y)))) in
-         f)%expr (at level 40, f at level 200, right associativity, format "'[' 'c.Mul128x128(' '$' n ','  x ','  y ')'  '<<'  count ';' ']' '//' f") : expr_scope.
-  Notation "'c.Add256(' '$' n ',' x ',' y ');' f" :=
-    (expr_let n := Z.cast2 (uint256, _)%core @@ (Z.add_get_carry_concrete $R @@ (x, y)) in
-         f)%expr (at level 40, f at level 200, right associativity, format "'[' 'c.Add256(' '$' n ','  x ','  y ');' ']' '//' f") : expr_scope.
-  Notation "'c.Add128(' '$' n ',' x ',' y ');' f" :=
-    (expr_let n := Z.cast2 (uint128, _)%core @@ (Z.add_get_carry_concrete $R @@ (x, y)) in
-         f)%expr (at level 40, f at level 200, right associativity, format "'[' 'c.Add128(' '$' n ','  x ','  y ');' ']' '//' f") : expr_scope.
-  Notation "'c.Add64(' '$' n ',' x ',' y ');' f" :=
-    (expr_let n := Z.cast uint128 @@ (Z.add @@ (x, y)) in
-         f)%expr (at level 40, f at level 200, right associativity, format "'[' 'c.Add64(' '$' n ','  x ','  y ');' ']' '//' f") : expr_scope.
-  Notation "'c.Addc256(' '$' n ',' x ',' y ',' z ');' f" :=
-    (expr_let n := Z.cast2 (uint256, _)%core @@ (Z.add_with_get_carry_concrete $R @@ (x, y, z)) in
-         f)%expr (at level 40, f at level 200, right associativity, format "'[' 'c.Addc256(' '$' n ','  x ','  y ','  z ');' ']' '//' f") : expr_scope.
-  Notation "'c.Addc128(' '$' n ',' x ',' y ',' z ');' f" :=
-    (expr_let n := Z.cast2 (uint128, _)%core @@ (Z.add_with_get_carry_concrete $R @@ (x, y, z)) in
-         f)%expr (at level 40, f at level 200, right associativity, format "'[' 'c.Addc128(' '$' n ','  x ','  y ','  z ');' ']' '//' f") : expr_scope.
-  Notation "'c.Selc(' '$' n ',' x ',' y ',' z ');' f" :=
-    (expr_let n := Z.cast uint256 @@ (Z.zselect @@ (x , y, z)) in
-         f)%expr (at level 40, f at level 200, right associativity, format "'[' 'c.Selc(' '$' n ','  x ','  y ','  z ');' ']' '//' f") : expr_scope.
-  Notation "'c.Selm(' '$' n ',' x ',' y ',' z ');' f" :=
-    (expr_let n := Z.cast uint256 @@ (Z.zselect @@ (Z.cast (r[0 ~>1]) @@ ((Z.cc_m_concrete _) @@ x), y, z)) in
-         f)%expr (at level 40, f at level 200, right associativity, format "'[' 'c.Selm(' '$' n ','  x ','  y ','  z ');' ']' '//' f") : expr_scope.
-  Notation "'c.Sell(' '$' n ',' x ',' y ',' z ');' f" :=
-    (expr_let n := Z.cast uint256 @@ (Z.zselect @@ (Z.cast (r[0~>1]) @@ (Z.land 1 @@ _ x), y, z)) in
-         f)%expr (at level 40, f at level 200, right associativity, format "'[' 'c.Sell(' '$' n ','  x ','  y ','  z ');' ']' '//' f") : expr_scope.
-  Notation "'c.Sub(' '$' n ',' x ',' y ');' f" :=
-    (expr_let n := Z.cast uint256 @@ (fst @@ (Z.cast2 (uint256, _)%core @@ (Z.sub_get_borrow_concrete $R @@ (x, y)))) in
-         f)%expr (at level 40, f at level 200, right associativity, format "'c.Sub(' '$' n ','  x ','  y ');' '//' f") : expr_scope.
-  Notation "'c.Sub(' '$' n ',' x ',' y ');' f" :=
-    (expr_let n := Z.cast2 (uint256, _)%core @@ (Z.sub_get_borrow_concrete $R @@ (x, y)) in
-         f)%expr (at level 40, f at level 200, right associativity, format "'c.Sub(' '$' n ','  x ','  y ');' '//' f") : expr_scope.
-  Notation "'c.AddM(' '$ret' ',' x ',' y ',' z ');'" :=
-    (Z.cast uint256 @@ (Z.add_modulo @@ (x, y, z)))%expr (at level 40, format "'c.AddM(' '$ret' ','  x ','  y ','  z ');'") : expr_scope.
-  Notation "'c.ShiftR(' '$' n ',' x ',' y ');' f" :=
-    (expr_let n := Z.cast _ @@ (Z.shiftr y @@ x) in f)%expr (at level 40, f at level 200, right associativity, format "'[' 'c.ShiftR(' '$' n ','  x ','  y ');' ']' '//' f") : expr_scope.
-  Notation "'c.Rshi(' '$' n ',' x ',' y ',' m ');' f" :=
-    (expr_let n := Z.cast _ @@ (Z.rshi_concrete $R m @@ (x, y)) in f)%expr (at level 40, f at level 200, right associativity, format "'[' 'c.Rshi(' '$' n ','  x ','  y ','  m ');' ']' '//' f") : expr_scope.
-  Notation "'c.ShiftL(' '$' n ',' x ',' y ');' f" :=
-    (expr_let n := Z.cast _ @@ (Z.shiftl y @@ x) in f)%expr (at level 40, f at level 200, right associativity, format "'[' 'c.ShiftL(' '$' n ','  x ','  y ');' ']' '//' f") : expr_scope.
-  Notation "'c.ShiftL(' '$' n ',' x ',' y ');' f" :=
-    (expr_let n := Z.cast _ @@ (Z.shiftl y @@ (Z.cast uint128 @@ (Z.land 340282366920938463463374607431768211455 @@ x))) in f)%expr (at level 40, f at level 200, right associativity, format "'[' 'c.ShiftL(' '$' n ','  x ','  y ');' ']' '//' f") : expr_scope.
-  Notation "'c.Lower128(' '$' n ',' x ');' f" :=
-    (expr_let n := Z.cast _ @@ (Z.land 340282366920938463463374607431768211455 @@ x) in f)%expr (at level 40, f at level 200, right associativity, format "'[' 'c.Lower128(' '$' n ','  x ');' ']' '//' f") : expr_scope.
-  Notation "'c.Lower(' x ')'"
-    := (Z.cast uint128 @@ (Z.land 340282366920938463463374607431768211455 @@ x))
-         (at level 10, only printing, format "c.Lower( x )")
-  : expr_scope.
-  Notation "'c.Upper(' x ')'"
-    := (Z.cast uint128 @@ (Z.shiftr 128 @@ x))
-         (at level 10, only printing, format "c.Upper( x )")
-  : expr_scope.
-  Notation "( v << count )"
-    := (Z.cast _ @@ (Z.shiftl count @@ v)%expr)
-         (format "( v  <<  count )")
-       : expr_scope.
-  (*
-  Notation "( x >> count )"
-    := (Z.cast _ @@ (Z.shiftr count @@ x)%expr)
-         (format "( x  >>  count )")
-       : expr_scope.
-  Notation "x * y"
-    := (Z.cast uint256 @@ (Z.mul @@ (x, y)))
-       : expr_scope.
-  *)
-End FancyPrintingNotations.
-
-
 Local Notation "i rd x y ; cont" := (Fancy.Instr i rd (x, y) cont) (at level 40, cont at level 200, format "i  rd  x  y ; '//' cont").
 Local Notation "i rd x y z ; cont" := (Fancy.Instr i rd (x, y, z) cont) (at level 40, cont at level 200, format "i  rd  x  y  z ; '//' cont").
 
 Import Fancy.Registers.
 Import Fancy.
+
+Import Barrett256 Montgomery256.
+
+(*** Montgomery Reduction ***)
+
+(* Status: Code in final form is proven correct modulo admits in compiler portions. *)
+
+(* Montgomery Code : *)
 Eval cbv beta iota delta [Prod.MontRed256 Prod.Mul256 Prod.Mul256x256] in Prod.MontRed256.
 (*
      = fun lo hi y t1 t2 scratch RegPInv : register =>
@@ -12330,46 +12515,107 @@ Eval cbv beta iota delta [Prod.MontRed256 Prod.Mul256 Prod.Mul256x256] in Prod.M
        ADDM lo lo RegZero RegMod;
        Ret lo
  *)
-Import Montgomery256.
+
+(* Uncomment to see proof statement and remaining admitted statements,
+or search for "prod_montred256_correct" to see comments on the proof
+preconditions. *)
+(* 
 Check Montgomery256.prod_montred256_correct.
-(* Print Assumptions Montgomery256.prod_montred256_correct. *)
+Print Assumptions Montgomery256.prod_montred256_correct.
+*)
 
-Import FancyPrintingNotations.
-Local Open Scope expr_scope.
+(*** Barrett Reduction ***)
 
-Print Barrett256.barrett_red256.
+(* Status : Code in "pre-fancy" (stage before final form) is proven
+correct modulo admits in compiler portions and one additional
+admit (see comment in barrett_red256_prefancy_correct). Code in final
+form ("fancy") is generated, but not yet proven equivalent to the
+"pre-fancy" version.
+
+The next step is to, using the same methodology as for Montgomery,
+prove the generated fancy code equivalent to Prod.MulMod and also
+equivalent to the "pre-fancy" code. Once these equivalences are
+proven, then the "pre-fancy" proof will apply to Prod.MulMod.
+ *)
+
+Import PreFancy.
+Import PreFancy.Notations.
+Local Notation "'RegMod'" := (Straightline.expr.Primitive (t:=type.Z) 115792089210356248762697446949407573530086143415290314195533631308867097853951).
+Local Notation "'RegMuLow'" := (Straightline.expr.Primitive (t:=type.Z) 26959946667150639793205513449348445388433292963828203772348655992835).
+
+(* "Prefancy" form : *)
+Print Barrett256.barrett_red256_prefancy.
 (*
-c.Selm($x0, $x_hi, RegZero, RegMuLow);
-c.Rshi($x1, RegZero, $x_hi, 255);
-c.Rshi($x2, $x_hi, $x_lo, 255);
-c.Mul128x128($x3, c.Upper(RegMuLow), c.Upper($x2));
-c.Mul128x128($x4, c.Upper(RegMuLow), c.Lower($x2));
-c.Mul128x128($x5, c.Lower(RegMuLow), c.Upper($x2));
-c.Mul128x128($x6, c.Lower(RegMuLow), c.Lower($x2));
-c.Add256($x7, (c.Lower($x4) << 128), $x6);
-c.Addc256($x8, $x7_hi, $x3, c.Upper($x5));
-c.Add256($x9, (c.Lower($x5) << 128), $x7_lo);
-c.Addc256($x10, $x9_hi, c.Upper($x4), $x8_lo);
-c.Add256($x11, $x2, $x10_lo);
-c.Addc128($x12, $x11_hi, RegZero, $x1);
-c.Add256($x13, $x0, $x11_lo);
-c.Addc128($x14, $x13_hi, RegZero, $x12_lo);
-c.Rshi($x15, $x14_lo, $x13_lo, 1);
-c.Mul128x128($x16, c.Upper(RegMod), c.Upper($x15));
-c.Mul128x128($x17, c.Lower(RegMod), c.Upper($x15));
-c.Mul128x128($x18, c.Upper(RegMod), c.Lower($x15));
-c.Mul128x128($x19, c.Lower(RegMod), c.Lower($x15));
-c.Add256($x20, (c.Lower($x17) << 128), $x19);
-c.Addc256($x21, $x20_hi, $x16, c.Upper($x18));
-c.Add256($x22, (c.Lower($x18) << 128), $x20_lo);
-c.Addc256($x23, $x22_hi, c.Upper($x17), $x21_lo);
-expr_let x24 := Z.add_get_carry_concrete
-                  115792089237316195423570985008687907853269984665640564039457584007913129639936 @@
-                (Z.opp @@ $x22_lo, $x_lo) in
-expr_let x25 := Z.add_with_get_carry_concrete
-                  115792089237316195423570985008687907853269984665640564039457584007913129639936 @@
-                ($x24_hi, Z.opp @@ $x23_lo, $x_hi) in
-c.Sell($x26, $x25_lo, RegZero, RegMod);
-c.Sub($x27, $x24_lo, $x26);
-c.AddM($ret, $x27, RegZero, RegMod);
+selm@(y, $x₂, RegZero, RegMuLow);
+rshi@(y0, RegZero, $x₂,255);
+rshi@(y1, $x₂, $x₁,255);
+mulhh@(y2, RegMuLow, $y1);
+mulhl@(y3, RegMuLow, $y1);
+mullh@(y4, RegMuLow, $y1);
+mulll@(y5, RegMuLow, $y1);
+add@(y6, $y5, $y4, 128);
+addc@(y7, carry{$y6}, $y2, $y4, -128);
+add@(y8, $y6, $y3, 128);
+addc@(y9, carry{$y8}, $y7, $y3, -128);
+add@(y10, $y1, $y9, 0);
+addc@(y11, carry{$y10}, RegZero, $y0, 0);
+add@(y12, $y, $y10, 0);
+addc@(y13, carry{$y12}, RegZero, $y11, 0);
+rshi@(y14, $y13, $y12,1);
+mulhh@(y15, RegMod, $y14);
+mullh@(y16, RegMod, $y14);
+mulhl@(y17, RegMod, $y14);
+mulll@(y18, RegMod, $y14);
+add@(y19, $y18, $y17, 128);
+addc@(y20, carry{$y19}, $y15, $y17, -128);
+add@(y21, $y19, $y16, 128);
+addc@(y22, carry{$y21}, $y20, $y16, -128);
+sub@(y23, $x₁, $y21, 0);
+subb@(y24, carry{$y23}, $x₂, $y22, 0);
+sell@(y25, $y24, RegZero, RegMod);
+sub@(y26, $y23, $y25, 0);
+addm@(y27, $y26, RegZero, RegMod);
+ret $y27
+ *)
+
+(* Uncomment to see proof statement and remaining admitted statements. *)
+(*
+Check barrett_red256_prefancy_correct.
+Print Assumptions barrett_red256_prefancy_correct.
+ *)
+
+(* "Fancy" code (NOT proven) *)
+Eval cbv beta iota delta [barrett_red256_alloc] in barrett_red256_alloc.
+(*
+     = fun (xLow xHigh RegMuLow : register) (_ : positive) (_ : register) =>
+       SELM r2 RegMuLow RegZero;
+       RSHI 255 r3 RegZero xHigh;
+       RSHI 255 r4 xHigh xLow;
+       MUL128UU r5 RegMuLow r4;
+       MUL128UL r6 r4 RegMuLow;
+       MUL128LU r7 r4 RegMuLow;
+       MUL128LL r8 RegMuLow r4;
+       ADD 128 r9 r8 r7;
+       ADDC (-128) r10 r5 r7;
+       ADD 128 r5 r9 r6;
+       ADDC (-128) r11 r10 r6;
+       ADD 0 r6 r4 r11;
+       ADDC 0 r12 RegZero r3;
+       ADD 0 r13 r2 r6;
+       ADDC 0 r14 RegZero r12;
+       RSHI 1 r15 r14 r13;
+       MUL128UU r16 RegMod r15;
+       MUL128LU r17 r15 RegMod;
+       MUL128UL r18 r15 RegMod;
+       MUL128LL r19 RegMod r15;
+       ADD 128 r20 r19 r18;
+       ADDC (-128) r21 r16 r18;
+       ADD 128 r22 r20 r17;
+       ADDC (-128) r23 r21 r17;
+       SUB 0 r24 xLow r22;
+       SUBC 0 r25 xHigh r23;
+       SELL r26 RegMod RegZero;
+       SUB 0 r27 r24 r26;
+       ADDM r28 r27 RegZero RegMod;
+       Ret r28
  *)
